code/chacha20poly1305/Hacl.Impl.Chacha20Poly1305.PolyCore.fst
@@ -1,6 +1,5 @@
 module Hacl.Impl.Chacha20Poly1305.PolyCore
 
-module ST = FStar.HyperStack.ST
 open FStar.HyperStack
 open FStar.HyperStack.All
 open FStar.Mul
@@ -9,11 +8,13 @@ open Lib.IntTypes
 open Lib.Buffer
 
 open Hacl.Impl.Poly1305.Fields
-open Hacl.Spec.Poly1305.Equiv
 
-module SpecPoly = Spec.Poly1305
+module ST = FStar.HyperStack.ST
 module Spec = Spec.Chacha20Poly1305
 module Poly = Hacl.Impl.Poly1305
+
+
+#set-options "--z3rlimit 50 --max_fuel 0 --max_ifuel 1"
 
 inline_for_extraction noextract
 let poly1305_padded_st (w:field_spec) =
@@ -21,19 +22,16 @@ let poly1305_padded_st (w:field_spec) =
   -> len:size_t
   -> text:lbuffer uint8 len ->
   Stack unit
-    (requires fun h ->
-      live h ctx /\ live h text /\ disjoint ctx text /\
-      Poly.state_inv_t h ctx)
-    (ensures fun h0 _ h1 ->
-      modifies (loc ctx) h0 h1 /\
-      Poly.state_inv_t h1 ctx /\
-      // Additional framing for r_elem
-      Poly.as_get_r h0 ctx == Poly.as_get_r h1 ctx /\
-      // Functional spec
-      Poly.as_get_acc h1 ctx ==
+  (requires fun h ->
+    live h ctx /\ live h text /\ disjoint ctx text /\
+    Poly.state_inv_t h ctx)
+  (ensures fun h0 _ h1 ->
+    modifies (loc ctx) h0 h1 /\
+    Poly.state_inv_t h1 ctx /\
+    Poly.as_get_r h0 ctx == Poly.as_get_r h1 ctx /\
+    Poly.as_get_acc h1 ctx ==
       Spec.poly1305_padded (Poly.as_get_r h0 ctx) (as_seq h0 text) (Poly.as_get_acc h0 ctx))
 
-#set-options "--z3rlimit 50 --max_fuel 0 --max_ifuel 1"
 
 inline_for_extraction noextract
 val poly1305_padded_: #w:field_spec -> poly1305_padded_st w
@@ -48,7 +46,6 @@ let poly1305_padded_ #w ctx len text =
   let rem = sub text (n *! 16ul) r in // the extra part of the input data
   Poly.poly1305_update #w ctx (n *! 16ul) blocks;
   let h2 = ST.get () in
-  poly_eq_lemma #(width w) (as_seq h1 blocks) (Poly.as_get_acc h1 ctx) (Poly.as_get_r h1 ctx);
   let tmp = create 16ul (u8 0) in
   update_sub tmp 0ul r rem;
   let h3 = ST.get() in
@@ -60,12 +57,14 @@ let poly1305_padded_ #w ctx len text =
   let h5 = ST.get () in
   Poly.reveal_ctx_inv ctx h4 h5
 
+
 [@CInline]
 let poly1305_padded_32 : poly1305_padded_st M32 = poly1305_padded_
 [@CInline]
 let poly1305_padded_128 : poly1305_padded_st M128 = poly1305_padded_
 [@CInline]
 let poly1305_padded_256 : poly1305_padded_st M256 = poly1305_padded_
+
 
 inline_for_extraction noextract
 val poly1305_padded: #w:field_spec -> poly1305_padded_st w
