code/chacha20poly1305/Hacl.Impl.Chacha20Poly1305.fsti
@@ -7,11 +7,13 @@ open FStar.HyperStack.All
 open Lib.IntTypes
 open Lib.Buffer
 
-module LSeq = Lib.Sequence
 module ST = FStar.HyperStack.ST
 module Spec = Spec.Chacha20Poly1305
 
 open Hacl.Impl.Poly1305.Fields
+
+
+#set-options "--z3rlimit 50 --max_fuel 0 --max_ifuel 1"
 
 inline_for_extraction noextract
 let aead_encrypt_st (w:field_spec) =
@@ -24,19 +26,21 @@ let aead_encrypt_st (w:field_spec) =
   -> output:lbuffer uint8 len
   -> tag:lbuffer uint8 16ul ->
   Stack unit
-    (requires (fun h ->
-      disjoint key output /\ disjoint nonce output /\
-      disjoint key tag /\ disjoint nonce tag /\
-      disjoint output tag /\
-      eq_or_disjoint input output /\
-      disjoint aad output /\
-      live h key /\ live h nonce /\ live h aad /\ live h input /\ live h output /\ live h tag))
-    (ensures  (fun h0 _ h1 -> modifies (loc output |+| loc tag) h0 h1 /\
-      Seq.append (as_seq h1 output) (as_seq h1 tag) ==
-      Spec.aead_encrypt (as_seq h0 key) (as_seq h0 nonce) (as_seq h0 input) (as_seq h0 aad)))
+  (requires fun h ->
+    live h key /\ live h nonce /\ live h aad /\
+    live h input /\ live h output /\ live h tag /\
+    disjoint key output /\ disjoint nonce output /\
+    disjoint key tag /\ disjoint nonce tag /\
+    disjoint output tag /\ eq_or_disjoint input output /\
+    disjoint aad output)
+  (ensures  fun h0 _ h1 -> modifies2 output tag h0 h1 /\
+    Seq.append (as_seq h1 output) (as_seq h1 tag) ==
+    Spec.aead_encrypt (as_seq h0 key) (as_seq h0 nonce) (as_seq h0 input) (as_seq h0 aad))
+
 
 inline_for_extraction noextract
 val aead_encrypt: #w:field_spec -> aead_encrypt_st w
+
 
 inline_for_extraction noextract
 let aead_decrypt_st (w:field_spec) =
@@ -49,17 +53,18 @@ let aead_decrypt_st (w:field_spec) =
   -> output:lbuffer uint8 len
   -> mac:lbuffer uint8 16ul ->
   Stack UInt32.t
-    (requires (fun h ->
-      eq_or_disjoint input output /\
-      live h key /\ live h nonce /\ live h aad /\ live h input /\ live h output /\ live h mac))
-    (ensures  (fun h0 z h1 -> modifies (loc input) h0 h1 /\
-      (let plain = Spec.aead_decrypt (as_seq h0 key) (as_seq h0 nonce) (as_seq h0 output) (as_seq h0 mac) (as_seq h0 aad) in
-      match z with
-      | 0ul -> Some? plain /\ as_seq h1 input == Some?.v plain // decryption succeeded
-      | 1ul -> None? plain
-      | _ -> false)  // decryption failed
-      )
-    )
+  (requires fun h ->
+    live h key /\ live h nonce /\ live h aad /\
+    live h input /\ live h output /\ live h mac /\
+    eq_or_disjoint input output)
+  (ensures  fun h0 z h1 -> modifies1 input h0 h1 /\
+   (let plain = Spec.aead_decrypt (as_seq h0 key) (as_seq h0 nonce) (as_seq h0 output) (as_seq h0 mac) (as_seq h0 aad) in
+    match z with
+    | 0ul -> Some? plain /\ as_seq h1 input == Some?.v plain // decryption succeeded
+    | 1ul -> None? plain
+    | _ -> false)  // decryption failed
+  )
+
 
 inline_for_extraction noextract
 val aead_decrypt: #w:field_spec -> aead_decrypt_st w
