code/poly1305/Lib.Loops.Lemmas.fsti
@@ -35,6 +35,23 @@ val repeati_right_extensionality:
     Loops.repeat_right lo_g (lo_g + n) (Loops.fixed_a a) g acc0))
 
 
+val repeat_blocks_multi_split:
+     #a:Type0
+  -> #b:Type0
+  -> size_block:size_pos
+  -> len0:nat{len0 % size_block = 0}
+  -> inp:seq a{len0 <= length inp /\ length inp % size_block = 0}
+  -> f:(lseq a size_block -> b -> b)
+  -> acc0:b ->
+  Lemma
+   (let len = length inp in
+    FStar.Math.Lemmas.modulo_addition_lemma len size_block (- len0 / size_block);
+    assert (len % size_block == (len - len0) % size_block);
+    repeat_blocks_multi size_block inp f acc0 ==
+    repeat_blocks_multi size_block (Seq.slice inp len0 len) f
+      (repeat_blocks_multi size_block (Seq.slice inp 0 len0) f acc0))
+
+
 val repeat_blocks_split:
      #a:Type0
   -> #b:Type0
@@ -50,23 +67,6 @@ val repeat_blocks_split:
     assert (len % size_block == (len - len0) % size_block);
     repeat_blocks size_block inp f l acc0 ==
     repeat_blocks size_block (Seq.slice inp len0 len) f l
-      (repeat_blocks_multi size_block (Seq.slice inp 0 len0) f acc0))
-
-
-val repeat_blocks_multi_split:
-     #a:Type0
-  -> #b:Type0
-  -> size_block:size_pos
-  -> len0:nat{len0 % size_block = 0}
-  -> inp:seq a{len0 <= length inp /\ length inp % size_block = 0}
-  -> f:(lseq a size_block -> b -> b)
-  -> acc0:b ->
-  Lemma
-   (let len = length inp in
-    FStar.Math.Lemmas.modulo_addition_lemma len size_block (- len0 / size_block);
-    assert (len % size_block == (len - len0) % size_block);
-    repeat_blocks_multi size_block inp f acc0 ==
-    repeat_blocks_multi size_block (Seq.slice inp len0 len) f
       (repeat_blocks_multi size_block (Seq.slice inp 0 len0) f acc0))
 
 
